theories/Block/vst/verif/certicoq_block__copy.v
@@ -6,7 +6,7 @@ From CertiCoq Require Import Block.vst.cmodel.certicoq_block_header.
 From CertiCoq Require Import Block.vst.cmodel.certicoq_block.
 From CertiCoq Require Import Block.vst.spec.spec.
 
-Lemma body: semax_body Vprog certicoq_block__specs.all f_certicoq_block__copy certicoq_block__copy_spec.
+Lemma body: semax_body Vprog certicoq_block__specs.gprog f_certicoq_block__copy certicoq_block__copy_spec.
 Proof.
   start_function.
   admit.
